steel/Learn.Steel.ListP.Param.fst
@@ -1,5 +1,6 @@
 module Learn.Steel.ListP.Param
 
+module G   = FStar.Ghost
 module US  = Learn.Steel.Util
 module Mem = Steel.Memory
 open Steel.Effect.Common
@@ -8,14 +9,18 @@ open Steel.Effect.Atomic
 open Steel.FractionalPermission
 open Steel.Reference
 
+#set-options "--ide_id_info_off"
+
+(* TODO *)
+irreducible let __ty_reduce__ : unit = ()
 
 noeq inline_for_extraction noextract
 type list_param_r' (r : Type) = {
   vp        : vprop;
-  data_t    : Type;
+  cdata_t   : Type;
   get_next  : normal (t_of vp) -> GTot (ref r);
   set_next  : normal (t_of vp) -> (nxt:ref r) -> GTot (c:normal (t_of vp) {get_next c == nxt});
-  get_data  : normal (t_of vp) -> GTot data_t;
+  get_data  : normal (t_of vp) -> GTot (normal cdata_t);
 
   read_next  : unit -> Steel (ref r) vp (fun _ -> vp) (requires fun _ -> True)
                       (ensures fun h0 x h1 -> frame_equalities vp h0 h1 /\ x == get_next (h0 vp));
@@ -33,7 +38,7 @@ type list_param_r (r : Type) = p:list_param_r' r {
      p.get_data (p.set_next s x) == p.get_data s)
 }
 
-noeq inline_for_extraction noextract
+noeq inline_for_extraction
 type list_param = {
   r      : Type;
   cell   : ref r -> list_param_r r;
@@ -42,7 +47,10 @@ type list_param = {
                  (ensures  is_null x == false)
 }
 
-let cell_t (p : list_param) : Type = x:ref p.r & (p.cell x).data_t
+[@@__ty_reduce__]
+let data_t (p : list_param) (x : ref p.r) : Type = (p.cell x).cdata_t
+[@@__ty_reduce__]
+let cell_t (p : list_param) : Type = dtuple2 (ref p.r) (data_t p)
 
 inline_for_extraction noextract
 let aptr_next (p : list_param) (x : ref p.r) : US.aptr (ref p.r) = {
@@ -66,7 +74,7 @@ let g_next (#q:vprop) (p:list_param) (x:ref p.r)
 [@@ __steel_reduce__]
 let g_data (#q:vprop) (p:list_param) (x:ref p.r)
   (h:rmem q{FStar.Tactics.with_tactic selector_tactic (can_be_split q (vcell p x) /\ True)})
-  : GTot ((p.cell x).data_t)
+  : GTot (data_t p x)
   = (p.cell x).get_data (h (vcell p x))
 
 [@@ __steel_reduce__]
@@ -84,8 +92,8 @@ let list_cell_not_null #opened (p : list_param) (x:ref p.r)
 
 
 inline_for_extraction noextract
-let list_param_of_vptr (c data_t : Type)
-    (gs_next : US.get_set_t c (ref c)) (get_data : c -> data_t)
+let list_param_of_vptr (c cdata_t : Type)
+    (gs_next : US.get_set_t c (ref c)) (get_data : c -> cdata_t)
   : Pure list_param
     (requires forall (s : c) (x:ref c) . {:pattern (get_data (gs_next.set s x))}
                 get_data (gs_next.set s x) == get_data s)
@@ -94,7 +102,7 @@ let list_param_of_vptr (c data_t : Type)
     r    = c;
     cell = (fun (r : ref c) -> {
               vp = vptr r;
-              data_t;
+              cdata_t;
               get_next = gs_next.get;
               set_next = (fun s x -> gs_next.set s x);
               get_data;
@@ -106,37 +114,82 @@ let list_param_of_vptr (c data_t : Type)
   }
 
 
-(* extending the vprop of a list_param *)
+(* [extend_list_param] : extending the vprop of a list_param *)
 
-let extend_list_param_vp1 (#r : Type) (p : list_param_r r) (ext : p.data_t -> vprop) (x : t_of (p.vp))
-  : vprop
-  = ext (p.get_data x)
+(* TODO? hide *)
 
-inline_for_extraction noextract
-let extend_list_param_r (r : Type) (p : list_param_r r) (ext : p.data_t -> vprop) : list_param_r r = {
-  vp         = p.vp `vdep` extend_list_param_vp1 p ext;
-  data_t     = x:p.data_t & (t_of (ext x));
-  get_next   = (fun (|x, y|) -> p.get_next x);
-  set_next   = (fun (|x, y|) nxt -> (|p.set_next x nxt, y|));
-  get_data   = (fun (|x, y|) -> (|p.get_data x, y|));
-  read_next  = (fun () ->
-                  (**) let sl = elim_vdep p.vp (extend_list_param_vp1 p ext) in
-                  let rt = p.read_next () in
-                  (**) intro_vdep p.vp (ext (p.get_data sl)) (extend_list_param_vp1 p ext);
-                  return rt);
-  write_next = (fun nxt ->
-                  (**) let sl = elim_vdep p.vp (extend_list_param_vp1 p ext) in
-                  p.write_next nxt;
-                  (**) intro_vdep p.vp (ext (p.get_data sl)) (extend_list_param_vp1 p ext));
+[@@erasable]
+noeq inline_for_extraction
+type list_param_ext_r (d0 : Type) = {
+  ext_vp     : d0 -> vprop;
+  ext_data_t : Type;
+  ext_data   : (x:d0) -> normal (t_of (ext_vp x)) -> GTot ext_data_t (* TODO? (x:d0 & ...) -> ... *)
 }
 
+type list_param_ext (p : list_param) : Type = (r : ref p.r) -> list_param_ext_r (data_t p r)
+
+let extend_list_param_vp1 (#r : Type) (p : list_param_r r) (e : list_param_ext_r p.cdata_t) (x : t_of (p.vp))
+  : vprop
+  = e.ext_vp (p.get_data x)
+
+[@@__ty_reduce__]
 inline_for_extraction noextract
-let extend_list_param (p : list_param) (ext : (r:ref p.r) -> (p.cell r).data_t -> vprop) : list_param = {
+let extend_list_param_r (r : Type) (p : list_param_r r) (e : list_param_ext_r p.cdata_t)
+  : list_param_r r = {
+  vp         = p.vp `vdep` extend_list_param_vp1 p e;
+  cdata_t    = e.ext_data_t;
+  get_next   = (fun (|x, y|) -> p.get_next x);
+  set_next   = (fun (|x, y|) nxt -> (|p.set_next x nxt, y|));
+  get_data   = (fun (|x, y|) -> e.ext_data (p.get_data x) y);
+  read_next  = (fun () ->
+                  (**) let sl = elim_vdep p.vp (extend_list_param_vp1 p e) in
+                  let rt = p.read_next () in
+                  (**) intro_vdep p.vp (e.ext_vp (p.get_data sl)) (extend_list_param_vp1 p e);
+                  return rt);
+  write_next = (fun nxt ->
+                  (**) let sl = elim_vdep p.vp (extend_list_param_vp1 p e) in
+                  p.write_next nxt;
+                  (**) intro_vdep p.vp (e.ext_vp (p.get_data sl)) (extend_list_param_vp1 p e));
+}
+
+[@@__ty_reduce__]
+inline_for_extraction noextract
+let extend_list_param (p : list_param) (e : list_param_ext p)
+  : list_param = {
   r     = p.r;
-  cell  = (fun (x : ref p.r) -> extend_list_param_r p.r (p.cell x) (ext x));
+  cell  = (fun (x : ref p.r) -> extend_list_param_r p.r (p.cell x) (e x));
   nnull = (fun (x : ref p.r) (m : Mem.mem) ->
-             interp_vdep_hp (p.cell x).vp (extend_list_param_vp1 (p.cell x) (ext x)) m;
+             interp_vdep_hp (p.cell x).vp (extend_list_param_vp1 (p.cell x) (e x)) m;
              p.nnull x m)
 }
 
-(* TODO: intro / elim *)
+let intro_ext_cell (#p : list_param) #opened (e : list_param_ext p) (r : ref p.r)
+                   (q : vprop)
+  : SteelGhost unit opened
+      (vcell p r `star` q) (fun () -> vcell (extend_list_param p e) r)
+      (requires fun h0 -> q == (e r).ext_vp (g_data p r h0))
+      (ensures  fun h0 () h1 ->
+        q == (e r).ext_vp (g_data p r h0) /\
+        g_data (extend_list_param p e) r h1
+          == (e r).ext_data (g_data p r h0) (h0 q) /\
+        g_next (extend_list_param p e) r h1
+          == g_next p r h0)
+  =
+    intro_vdep (vcell p r) q (extend_list_param_vp1 (p.cell r) (e r))
+
+let elim_ext_cell (#p : list_param) #opened (e : list_param_ext p) (r : ref p.r)
+  : SteelGhost (G.erased (data_t p r)) opened
+      (vcell (extend_list_param p e) r) (fun dt -> vcell p r `star` (e r).ext_vp dt)
+      (requires fun _ -> True)
+      (ensures  fun h0 dt h1 ->
+         G.reveal dt == g_data p r h1 /\
+         g_data (extend_list_param p e) r h0
+           == (e r).ext_data dt (h1 ((e r).ext_vp dt)) /\
+         g_next (extend_list_param p e) r h0
+           == g_next p r h1)
+  =
+    let sl = elim_vdep (vcell p r) (extend_list_param_vp1 (p.cell r) (e r)) in
+    let dt : G.erased (data_t p r) = (p.cell r).get_data sl in
+    change_equal_slprop (extend_list_param_vp1 (p.cell r) (e r) sl)
+                        ((e r).ext_vp dt);
+    dt
