steel/Learn.Steel.ListP.Test.fst
@@ -1,7 +1,9 @@
 module Learn.Steel.ListP.Test
 
+module U   = Learn.Util
 module L   = FStar.List.Pure
 module G   = FStar.Ghost
+module Ll  = Learn.List
 module US  = Learn.Steel.Util
 module U32 = FStar.UInt32
 
@@ -10,6 +12,8 @@ open Steel.Effect.Atomic
 open Steel.Reference
 
 open Learn.Steel.ListP
+
+#set-options "--ide_id_info_off"
 
 #push-options "--__no_positivity"
 noeq
@@ -59,14 +63,11 @@ let p1 : list_param =
     ({get = (fun c -> c.next); set = (fun c x -> {c with next = x})})
     (fun c   -> c.data_p)
 
-noextract
-type p1_ext = (r : ref cell1) -> ref U32.t -> vprop
-
 inline_for_extraction noextract
-let p1' (ext : p1_ext) : list_param
+let p1' (ext : list_param_ext p1) : list_param
   = extend_list_param p1 ext
 
-let rec p1_length (ext : p1_ext) (r : ref cell1)
+let rec p1_length (ext : list_param_ext p1) (r : ref cell1)
   : Steel  U32.t
           (mlistN (p1' ext) r) (fun _ -> mlistN (p1' ext) r)
           (requires fun h0        -> L.length (sel_listN (p1' ext) r h0) <= FStar.UInt.max_int U32.n)
@@ -74,10 +75,14 @@ let rec p1_length (ext : p1_ext) (r : ref cell1)
                                   U32.v len = L.length (sel_listN (p1' ext) r h0))
   = length_body (p1' ext) (p1_length ext) r
 
-noextract
-let p1_ext0 : p1_ext = fun _ _ -> emp
-noextract
-let p1_ext1 : p1_ext = fun _ r -> vptr r
+inline_for_extraction
+let p1_ext0 : list_param_ext p1 =
+  fun _ -> {ext_vp = (fun _ -> emp); ext_data_t = ref U32.t; ext_data = (fun r _ -> r)}
+inline_for_extraction
+let p1_ext1 : list_param_ext p1 =
+  fun _ -> { ext_vp = (fun r -> vptr r);
+          ext_data_t = (ref U32.t & U32.t);
+          ext_data = (fun r x -> (r,x))}
 
 let test_p1_ext0 (l : ref cell1)
   : Steel bool (mlistN (p1' p1_ext0) l) (fun _ -> mlistN (p1' p1_ext0) l)
@@ -93,25 +98,27 @@ let test_p1_ext1 (l : ref cell1)
                 (ensures  fun h0 rt h1 ->
                   frame_equalities (mlistN (p1' p1_ext1) l) h0 h1 /\
                  (let lv = sel_listN (p1' p1_ext1) l h0 in
-                  (rt <> 0ul ==> Cons? lv /\ (L.hd lv)._2._2 == rt)))
+                  (rt <> 0ul ==> Cons? lv /\ (L.hd lv <: (x:ref cell1 & (ref U32.t & U32.t)))._2._2 == rt)))
   =
     let len = p1_length p1_ext1 l in
     if U32.(len >^ 0ul)
     then begin
       (**) let lv = gget (mlistN (p1' p1_ext1) l) in
       (**) let r1 = elim_mlistN_cons (p1' p1_ext1) l (L.hd lv) (L.tl lv) in
-      (**) let g_cl = elim_vdep (vptr l) (extend_list_param_vp1 (p1.cell l) (p1_ext1 l)) in
+      (**) let g_ptr = elim_ext_cell p1_ext1 l in
       let cl = read l in 
-      (**) assert (G.reveal g_cl == cl);
-      (**) change_equal_slprop (vptr g_cl.data_p) (vptr cl.data_p);
+      (**) assert (G.reveal g_ptr == cl.data_p);
+      (**) change_equal_slprop (vptr g_ptr) (vptr cl.data_p);
       let rt = read cl.data_p in
-      (**) intro_vdep (vptr l) (vptr cl.data_p) (extend_list_param_vp1 (p1.cell l) (p1_ext1 l));
+      (**) intro_ext_cell p1_ext1 l (vptr cl.data_p);
       (**) intro_mlistN_cons (p1' p1_ext1) l r1;
       return rt
     end else return 0ul
 
 
 (* ------------------------------------------------------------------- *)
+
+module Mem = Steel.Memory
 
 #push-options "--__no_positivity"
 noeq
@@ -122,43 +129,211 @@ type cell2 = {
 }
 #pop-options
 
-(* TODO? [@@ erasable] on list_param *)
 inline_for_extraction noextract
 let p2_0 : list_param =
   list_param_of_vptr cell2 (ghost_ref bool & ref U32.t)
     ({get = (fun c -> c.next); set = (fun c x -> {c with next = x})})
     (fun c   -> (c.data_b, c.data_p))
 
-noextract
-let p2_ext ((b, p) : (ghost_ref bool & ref U32.t)) : vprop =
-  ghost_vptr b `vdep` (fun b -> US.vopt b (vptr p))
+noeq noextract
+type p2_data_t = {
+  ref_b : ghost_ref bool;
+  ref_p : ref U32.t;
+  p_val : option U32.t
+}
 
+[@@__ty_reduce__]
+inline_for_extraction
+let p2_ext : list_param_ext_r (ghost_ref bool & ref U32.t) = {
+  ext_vp     = (fun (rs : ghost_ref bool & ref U32.t) ->
+                  ghost_vptr rs._1 `vdep` (fun b -> US.vopt b (vptr rs._2)));
+  ext_data_t = p2_data_t;
+  ext_data   = (fun (ref_b, ref_p) (|_, p_val|) -> {ref_b;ref_p;p_val})
+}
+
+[@@__ty_reduce__]
 inline_for_extraction noextract
 let p2 = extend_list_param p2_0 (fun _ -> p2_ext)
 
-(* TODO
-assume
-val extract_data_p (#opened : Mem.inames) (c : ref cell2) (rp : ref U32.t)
-  : unit -> SteelGhost unit opened
+let p2_data_extract (#opened : Mem.inames) (c : ref cell2) (rp : ref U32.t)
+  : SteelGhost unit opened
       (vcell p2 c) (fun () -> vcell p2 c `star` vptr rp)
-      (requires fun h0       -> let (|(_, rp'), (|b, _|)|) = g_data p2 c h0 in
-                             (b <: bool) /\ rp' == rp)
+      (requires fun h0       -> let d0 = g_data p2 c h0 in
+                             d0.ref_p == rp /\ Some? d0.p_val)
       (ensures  fun h0 () h1 -> g_next p2 c h1 == g_next p2 c h0 /\
-                            (let (|(rb, rp'), _|) = g_data p2 c h0 in
-                             g_data p2 c h1 == (|(rb, rp'), (|false, None #U32.t|)|)))
+                            (let d0 = g_data p2 c h0 in
+                             Some? d0.p_val /\
+                             g_data p2 c h1 == {d0 with p_val = None} /\
+                             sel rp h1 == Some?.v d0.p_val))
+ =
+   let g_rs = elim_ext_cell (fun _ -> p2_ext) c in
+   let (r_b, r_p) : ghost_ref bool & ref U32.t = G.reveal g_rs in
+   assert_norm (p2_ext.ext_vp (r_b, r_p)
+             == ghost_vptr r_b `vdep` (fun b -> US.vopt b (vptr r_p)));
+   change_equal_slprop (p2_ext.ext_vp g_rs)
+                       (ghost_vptr r_b `vdep` (fun b -> US.vopt b (vptr r_p)));
+   let g_b = elim_vdep (ghost_vptr r_b) (fun b -> US.vopt b (vptr r_p)) in
+   assert (g_b <: bool);
+   US.vopt_elim_t (vptr r_p);
+   change_equal_slprop (vptr r_p) (vptr rp);
 
-let test_p2 (l : ref cell2) (len : G.erased nat) (r1 : ref U32.t)
-  : Steel unit (mlist p2 l len null) (fun () -> mlist p2 l len null `star` vptr r1)
-               (requires fun h0 -> len >= 2 /\
-                               (let (|_, (|(_,r1'), (|b, _|)|)|) = L.index (sel_list p2 l len null h0) 1
-                                in (b <: bool) /\ r1' == r1))
-               (ensures fun h0 () h1 -> True)
+   US.vopt_intro_f (vptr r_p);
+   ghost_write r_b false;
+   intro_vdep (ghost_vptr r_b)
+              (US.vopt false (vptr r_p))
+              (fun b -> US.vopt b (vptr r_p));
+   intro_ext_cell (fun _ -> p2_ext) c 
+                  (ghost_vptr r_b `vdep` (fun b -> US.vopt b (vptr r_p)))
+
+let p2_data_insert (#opened : Mem.inames) (c : ref cell2) (rp : ref U32.t)
+  : SteelGhost unit opened
+      (vcell p2 c `star` vptr rp) (fun () -> vcell p2 c)
+      (requires fun h0       -> let d0 = g_data p2 c h0 in
+                             d0.ref_p == rp /\ None? d0.p_val)
+      (ensures  fun h0 () h1 -> g_next p2 c h1 == g_next p2 c h0 /\
+                            (let d0 = g_data p2 c h0 in
+                             g_data p2 c h1 == {d0 with p_val = Some (sel rp h0)}))
+ =
+   let g_rs = elim_ext_cell (fun _ -> p2_ext) c in
+   let (r_b, r_p) : ghost_ref bool & ref U32.t = G.reveal g_rs in
+   assert_norm (p2_ext.ext_vp (r_b, r_p)
+             == ghost_vptr r_b `vdep` (fun b -> US.vopt b (vptr r_p)));
+   change_equal_slprop (p2_ext.ext_vp g_rs)
+                       (ghost_vptr r_b `vdep` (fun b -> US.vopt b (vptr r_p)));
+   let g_b = elim_vdep (ghost_vptr r_b) (fun b -> US.vopt b (vptr r_p)) in
+   assert (not g_b);
+   US.vopt_elim_f (vptr r_p);
+   
+   change_equal_slprop (vptr rp) (vptr r_p);
+   US.vopt_intro_t (vptr r_p);
+   ghost_write r_b true;
+   intro_vdep (ghost_vptr r_b)
+              (US.vopt true (vptr r_p))
+              (fun b -> US.vopt b (vptr r_p));
+   intro_ext_cell (fun _ -> p2_ext) c 
+                  (ghost_vptr r_b `vdep` (fun b -> US.vopt b (vptr r_p)))
+
+
+let rec p2_index (r : ref cell2) (len : G.erased nat) (exit : G.erased (ref cell2)) (i : U32.t)
+  : Steel (ref cell2)
+          (mlist p2 r len exit) (fun _ -> mlist p2 r len exit)
+          (requires fun h -> U32.v i < len)
+          (ensures  fun h rt h' -> U32.v i < len /\
+                          frame_equalities (mlist p2 r len exit) h h' /\
+                          rt == (L.index (sel_list p2 r len exit h) (U32.v i))._1)
+  = index_body p2 p2_index r len exit i
+
+
+(* TODO *)
+noextract unfold
+let normal_ty_steps =
+   [delta_attr [`%__ty_reduce__];
+    delta_only [`%Mklist_param?.cell;
+                `%Mklist_param_r'?.cdata_t;
+                `%Mklist_param_ext_r?.ext_data_t];
+    iota]
+
+inline_for_extraction noextract unfold
+let normal_ty (#a:Type) (x:a) = norm normal_ty_steps x
+
+
+#push-options "--ifuel 0"
+let p2_data_extract_nth #opened (l : ref cell2) (len : nat) (exit : ref cell2) (i : nat) (r_p : ref U32.t)
+  : SteelGhost unit opened
+      (mlist p2 l len exit) (fun () -> mlist p2 l len exit `star` vptr r_p)
+      (requires fun h0 -> i < len /\
+                      (let d0 = (L.index (sel_list p2 l len exit h0) i)._2 in
+                       d0.ref_p == r_p /\ Some? d0.p_val))
+      (ensures fun h0 () h1 ->
+                       i < len /\
+                      (let l0 = sel_list p2 l len exit h0 in
+                       let cl0 = L.index l0 i in
+                       let ri = cl0._1 in let d0 = cl0._2 in
+                       sel_list p2 l len exit h1 == Ll.set i ((|ri, {d0 with p_val = None}|)) l0 /\
+                       Some? d0.p_val /\
+                       sel r_p h1 == Some?.v d0.p_val))
   =
-    let lv : G.erased (mlist_sel_t p2 l len null) = gget (mlist p2 l len null) in
-    let d0_r = G.hide (L.index lv 1)._1 in
-    let d0   = G.hide ((L.index lv 1)._2
-                      <: dtuple2 (ghost_ref bool & ref U32.t) (fun (_,_) -> (_:bool & option U32.t)) )in
-    mlist_gmap_at p2 l len null 1 (L.index lv 1)._1 d0 (|dfst (G.reveal d0), (|false, None #U32.t|)|)
-      emp (vptr r1) (fun (_ : t_of emp) -> True) (fun _ -> True)
-      (extract_data_p (L.index lv 1)._1 r1)
-*)
+    let lv : G.erased (mlist_sel_t p2 l len exit) = gget (mlist p2 l len exit) in
+    let (|r_i,d0|) : x:ref cell2 & data_t p2 x = L.index lv i in
+    let d1  = {U.cast p2_data_t d0 with p_val = None} in
+    mlist_gmap_at p2 l len exit i r_i d0 d1
+      emp (vptr r_p) (fun (_ : t_of emp) -> True) (fun (_ : t_of emp) (x : U32.t) -> x == Some?.v d0.p_val)
+      (fun () -> p2_data_extract r_i r_p)
+
+let p2_data_insert_nth #opened (l : ref cell2) (len : nat) (exit : ref cell2) (i : nat) (rpi : ref U32.t)
+  : SteelGhost unit opened
+      (mlist p2 l len exit `star` vptr rpi) (fun () -> mlist p2 l len exit)
+      (requires fun h0 -> i < len /\
+                      (let d0 = (L.index (sel_list p2 l len exit h0) i)._2 in
+                       d0.ref_p == rpi /\ None? d0.p_val))
+      (ensures fun h0 () h1 ->
+                       i < len /\
+                      (let l0 = sel_list p2 l len exit h0 in
+                       let cl0 = L.index l0 i in
+                       let ri = cl0._1 in let d0 = cl0._2 in
+                       sel_list p2 l len exit h1
+                         == Ll.set i ((|ri, {d0 with p_val = Some (sel rpi h0)}|)) l0))
+  =
+    let lv : G.erased (mlist_sel_t p2 l len exit) = gget (mlist p2 l len exit) in
+    let x  : G.erased U32.t = gget (vptr rpi) in
+    let (|r_i,d0|) : x:ref cell2 & data_t p2 x = L.index lv i in
+    let d1  = {U.cast p2_data_t d0 with p_val = Some (G.reveal x)} in
+    mlist_gmap_at p2 l len exit i r_i d0 d1
+      (vptr rpi) emp (fun x' -> x' == G.reveal x) (fun _ _ -> True)
+      (fun () -> p2_data_insert r_i rpi)
+
+
+inline_for_extraction noextract
+let p2_extract_index (l : ref cell2) (len : G.erased nat) (exit : G.erased (ref cell2)) (i : U32.t)
+  : Steel (ref U32.t)
+      (mlist p2 l len exit) (fun r_p -> mlist p2 l len exit `star` vptr r_p)
+      (requires fun h0 -> U32.v i < len /\
+                       Some? (L.index (sel_list p2 l len exit h0) (U32.v i))._2.p_val)
+      (ensures fun h0 r_p h1 ->
+                       U32.v i < len /\
+                      (let l0  = sel_list p2 l len exit h0 in
+                       let cl0 = L.index l0 (U32.v i) in
+                       let ri = cl0._1 in let d0 = cl0._2 in
+                       r_p == d0.ref_p /\
+                       sel_list p2 l len exit h1
+                         == Ll.set (U32.v i) ((|ri, {d0 with p_val = None}|)) l0 /\
+                       Some? d0.p_val /\
+                       sel r_p h1 == Some?.v d0.p_val))
+  =
+    let r  = p2_index l len exit i in
+    (**) let ex = mlist_extract p2 l len exit (U32.v i) in
+    (**) change_equal_slprop (vcell p2 ex.r) (vcell p2 r);
+    (**) let g_rs = elim_ext_cell #p2_0 (fun _ -> p2_ext) r in
+    let cl  = read r in
+    let r_p = cl.data_p in
+    (**) intro_ext_cell #p2_0 (fun _ -> p2_ext) r (p2_ext.ext_vp g_rs);
+    (**) p2_data_extract r r_p;
+    (**) change_equal_slprop (vcell p2 r) (vcell p2 ex.r);
+    (**) ex.close ();
+    return r_p
+#pop-options
+
+let test_p2 (l : ref cell2) (len : G.erased nat) (exit : G.erased (ref cell2)) (i0 i1 : U32.t)
+  : Steel unit
+      (mlist p2 l len exit) (fun () -> mlist p2 l len exit)
+      (requires fun h0 -> U32.v i0 < len /\ U32.v i1 < len /\ U32.(v i0 <> v i1) /\
+                      (let l0 = sel_list p2 l len exit h0 in
+                       Some? (L.index l0 (U32.v i0))._2.p_val /\
+                       Some? (L.index l0 (U32.v i1))._2.p_val))
+      (ensures fun h0 () h1 ->
+                       U32.v i0 < len /\ U32.v i1 < len /\
+                      (let l0 = sel_list p2 l len exit h1 in
+                       Some? (L.index l0 (U32.v i0))._2.p_val /\
+                       Some? (L.index l0 (U32.v i1))._2.p_val))
+  =
+    let r0 = p2_extract_index l len exit i0 in
+    let r1 = p2_extract_index l len exit i1 in
+    write r0 0ul;
+    write r1 1ul;
+    (* TODO: extract
+    let _ = par
+      (fun () -> (write r0 0ul <: SteelT unit (vptr r0) (fun () -> vptr r0)))
+      (fun () -> (write r1 1ul <: SteelT unit (vptr r1) (fun () -> vptr r1))) in
+     *)
+    (**) p2_data_insert_nth l len exit (U32.v i0) r0;
+    (**) p2_data_insert_nth l len exit (U32.v i1) r1
